tactics: fix quote
need to mark it unfold, otherwise its argument might reduce when `quote`
is not expanded into an `__embed`.

For example, in this code

	let _ = assert_by_tactic (t <-- quote ((x:int) -> x == 2 /\ False);
				  match term_as_formula t with
				  | Forall _ _ -> return ()
				  | _ -> fail ("This should be a forall: " ^ term_to_string t)) True

`x == 2 /\ False` was being normalized (/ simplified) to False.

This might not be a very great solution.

ulib/FStar.Tactics.fst
@@ -101,7 +101,7 @@ let or_else (#a:Type) (t1 : tactic a) (t2 : tactic a) : tactic a =
  * assume __embed as a `a -> tactic term` computation (TODO?)
  *)
 assume private val __embed  : #a:Type -> a -> term
-let quote #a (x:a) : tactic term = fun () -> __embed x
+unfold let quote #a (x:a) : tactic term = fun () -> __embed x
 
 
 (* Many of these could be derived from apply_lemma,
